\section{Si $p \in \mathbb{Z}$ es primo y $a^2 \stackrel{p}{\equiv} b^2$, entonces $a \stackrel{p}{\equiv} b$ o $-a \stackrel{p}{\equiv} -b$}
 \begin{proof}

    Si p $\in \mathbb{Z}$  es primo y a^2 $\stackrel{p}{ \equiv } b^2$ \\
   $a^2-b^2 = pk$,  $k \in \mathbb{Z}$
   \begin{align}
        \notag (a+b)(a-b)= pk\\
        \notag a+b = 0=p(0)\\
        \notag \therefore a \stackrel{p}{ \equiv } = -b\\
   \end{align}

   Si $a-b = 0=p(0)$\\
   $\therefore a \stackrel{p}{ \equiv } = b$\\
    Si $a+b \neq 0 \land a-b \neq $\\
    Si  $a+b= p  \lor a-b = p\\$
    \begin{align}
    \notag \therefore p | a \lor p | b \\
    \notag \therefore a\stackrel{p}{ \equiv } 0 \stackrel{p}{ \equiv } \\
    \end{align}

    Si $ a+b \neq p  \land a-b \neq p$ \\
    \begin{align}
\notag \therefore \frac{k}{a+b}, \frac{k}{a-b} \in \mathbb{Z}\\
    \therefore a+b = pk \lor a-b = pk \\
    \notag y \therefore a\stackrel{p}{ \equiv }-b \ \lor 
    \notag \stackrel{p}{ \equiv } b
    \end{align} \

 \end{proof}